src/tactics/FStar.Tactics.Types.fsti
@@ -124,6 +124,6 @@ type unfold_side =
   | Both
   | Neither
 
-type effect_label =
+type tot_or_ghost =
   | E_Total
   | E_Ghost
